tests/lean/Tutorial/Proofs.lean
@@ -224,4 +224,519 @@ def use_counter
   (T : Type) (CounterInst : Counter T) (cnt : T) : Result (Usize × T) :=
   CounterInst.incr cnt
 
+
+/- [tutorial::zero]: loop 0:
+   Source: 'src/lib.rs', lines 6:4-11:1 -/
+divergent def zero_loop
+  (x : alloc.vec.Vec U32) (i : Usize) : Result (alloc.vec.Vec U32) :=
+  let i1 := alloc.vec.Vec.len U32 x
+  if i < i1
+  then
+    do
+    let (_, index_mut_back) ←
+      alloc.vec.Vec.index_mut U32 Usize
+        (core.slice.index.SliceIndexUsizeSliceTInst U32) x i
+    let i2 ← i + 1#usize
+    let x1 ← index_mut_back 0#u32
+    zero_loop x1 i2
+  else Result.ok x
+
+-- TODO:
+@[simp, scalar_tac ls.update i x]
+theorem length_update (ls : List α) (i : Int) (x : α) : (ls.update i x).length = ls.length := by
+  sorry
+
+@[scalar_tac l0 = l1]
+theorem List.eq_imp_length_eq (l0 l1 : List α) : l0 = l1 → l0.length = l1.length := by intro; simp [*]
+
+-- TODO:
+@[scalar_tac ls0 = ls1]
+theorem list_eq_imp_length_eq {α : Type u} (ls0 ls1 : List α) (h : ls0 = ls1) :
+  ls0.length = ls1.length := by
+  scalar_tac_preprocess
+  simp [*]
+
+set_option maxHeartbeats 1000000
+
+-- TODO: this doesn't work
+@[simp]
+theorem index_update_eq_unsigned_scalar
+  {α : Type u} [Inhabited α] (l: List α) (i: Scalar ty) (x: α) :
+  ¬ ty.isSigned → i.val < l.length → (l.update i.val x).index i.val = x := by
+  intros
+  apply List.index_update_eq <;> (try simp [*])
+  cases ty <;> simp_all <;> scalar_tac
+
+abbrev Bignum U32 := alloc.vec.Vec U32
+
+@[simp]
+def toInt_aux (l : List U32) : ℤ :=
+  match l with
+  | [] => 0
+  | x :: l =>
+    x + 2 ^ 32 * toInt_aux l
+
+@[reducible]
+def toInt (x : alloc.vec.Vec U32) : ℤ := toInt_aux x.val
+
+@[pspec]
+theorem zero_loop_spec
+  (x : alloc.vec.Vec U32) (i : Usize) (h : i.val ≤ x.length) :
+  ∃ x',
+    zero_loop x i = ok x' ∧
+    x'.length = x.length ∧
+    (∀ j, 0 ≤ j → j < i.val → x'.val.index j = x.val.index j) ∧
+    (∀ j, i.val ≤ j → j < x.length → x'.val.index j = 0#u32) := by
+  rw [zero_loop]
+  simp
+  split
+  . progress as ⟨ _ ⟩
+    progress as ⟨ i1 ⟩
+    progress as ⟨ x1 ⟩
+    progress as ⟨ x2, _, hSame, hZero ⟩
+    . -- TODO: we should use scalar_tac here
+      scalar_tac_preprocess
+      simp_all
+      omega
+    . simp_all
+      split_conjs
+      . intro j h0 h1
+        replace hSame := hSame j (by scalar_tac) (by scalar_tac)
+        simp_all
+      . intro j h0 h1
+        -- TODO: we want a shortcut for this
+        cases h: (¬ j = i.val : Bool) <;> simp_all
+        . have := hSame j (by scalar_tac) (by scalar_tac)
+          simp_all
+        . apply hZero j (by scalar_tac) (by scalar_tac)
+  . simp; scalar_tac
+termination_by (x.length - i.val).toNat
+decreasing_by scalar_decr_tac
+
+/- [tutorial::zero]:
+   Source: 'src/lib.rs', lines 5:0-5:28 -/
+def zero (x : alloc.vec.Vec U32) : Result (alloc.vec.Vec U32) :=
+  zero_loop x 0#usize
+
+theorem all_nil_impl_toInt_eq_zero
+  (l : List U32) (h : ∀ (j : ℕ), j < l.length → l.index j = 0#u32) :
+  toInt_aux l = 0 := by
+  match l with
+  | [] => simp
+  | hd :: tl =>
+    have h1 := h 0
+    simp_all
+    apply all_nil_impl_toInt_eq_zero
+    intro j h2
+    have := h (j + 1)
+    simp_all
+
+theorem zero_spec (x : alloc.vec.Vec U32) :
+  ∃ x',
+    zero x = ok x' ∧
+    x'.length = x.length ∧
+    toInt x' = 0 := by
+    rw [zero]
+    progress as ⟨ x', hLength, hSame, hZero ⟩
+    simp_all
+    apply all_nil_impl_toInt_eq_zero
+    simp_all
+
+/- [tutorial::add_no_overflow]: loop 0:
+   Source: 'src/lib.rs', lines 19:4-24:1 -/
+divergent def add_no_overflow_loop
+  (x : alloc.vec.Vec U32) (y : alloc.vec.Vec U32) (i : Usize) :
+  Result (alloc.vec.Vec U32)
+  :=
+  let i1 := alloc.vec.Vec.len U32 x
+  if i < i1
+  then
+    do
+    let i2 ←
+      alloc.vec.Vec.index U32 Usize (core.slice.index.SliceIndexUsizeSliceTInst
+        U32) y i
+    let (i3, index_mut_back) ←
+      alloc.vec.Vec.index_mut U32 Usize
+        (core.slice.index.SliceIndexUsizeSliceTInst U32) x i
+    let i4 ← i3 + i2
+    let i5 ← i + 1#usize
+    let x1 ← index_mut_back i4
+    add_no_overflow_loop x1 y i5
+  else Result.ok x
+
+#check List.splitAtD
+#check List.slice
+
+@[simp]
+def List.isplitAt (l : List α) (i : ℤ) : List α × List α :=
+  match l with
+  | [] => ([], [])
+  | hd :: tl =>
+    if i = 0 then ([], hd :: tl)
+    else
+      let (l0, l1) := isplitAt tl (i - 1)
+      (hd :: l0, l1)
+
+-- Here, we're using ring_nf
+@[simp]
+theorem toInt_aux_append (l0 l1 : List U32) :
+  toInt_aux (l0 ++ l1) = toInt_aux l0 + 2 ^ (32 * l0.length) * toInt_aux l1 := by
+  match l0 with
+  | [] => simp
+  | hd :: tl =>
+    have := toInt_aux_append tl l1
+    simp_all
+    ring_nf
+
+-- TODO: specialize the theorems for the cases unsigned scalar
+-- Ex.: (x.val + n).toNat = x.toNat + n.toNat
+@[simp]
+theorem toInt_aux_update (l : List U32) (i : Int) (x : U32) (h0 : 0 ≤ i) (h1 : i < l.length) :
+  toInt_aux (l.update i x) = toInt_aux l + 2 ^ (32 * i.toNat) * (x - l.index i) := by
+  cases l with
+  | nil => simp at *; scalar_tac
+  | cons hd tl =>
+    simp_all
+    -- TODO: simplify this
+    cases h : (i = 0 : Bool) <;> simp_all
+    . have := toInt_aux_update tl (i - 1) x (by scalar_tac) (by scalar_tac)
+      simp_all
+      ring_nf at *
+      simp [← add_assoc] -- TODO
+      have : (2 ^ ((i.toNat - 1) * 32) * 4294967296  : Int) = 2 ^ (32 * i.toNat) := by
+        ring_nf
+        have : i.toNat = i.toNat - 1 + 1 := by scalar_tac
+        conv => rhs; rw [this]
+        ring_nf
+      simp [mul_assoc, *]
+      ring_nf
+    . ring_nf
+
+@[simp]
+theorem toInt_aux_idrop (l : List U32) (i : Int) (h0 : 0 ≤ i) (h1 : i < l.length) :
+  toInt_aux (l.idrop i) = l.index i + 2 ^ 32 * toInt_aux (l.idrop (i + 1)) := by
+  cases l with
+  | nil => simp at *; scalar_tac
+  | cons hd tl =>
+    simp_all
+    -- TODO: simplify this
+    cases h : (i = 0 : Bool) <;> simp_all
+    have := toInt_aux_idrop tl (i - 1) (by scalar_tac) (by scalar_tac)
+    simp_all
+    ring_nf at *
+    have : 0 < 1 + i := by scalar_tac
+    simp [*]
+
+@[simp]
+theorem UScalar.add_nat_toNat (h : ¬ ty.isSigned) (x : Scalar ty) (n : Nat) :
+  (x.val + n).toNat = x.val.toNat + n := by
+  cases ty <;> simp_all <;> scalar_tac
+
+@[simp]
+theorem UScalar.nat_add_toNat (h : ¬ ty.isSigned) (x : Scalar ty) (n : Nat) :
+  (n + x.val).toNat = x.val.toNat + n := by
+  cases ty <;> simp_all <;> scalar_tac
+
+@[simp]
+theorem UScalar.add_pos_toNat (h : ¬ ty.isSigned) (x : Scalar ty) (n : Int) (h' : 0 ≤ n) :
+  (x.val + n).toNat = x.val.toNat + n.toNat := by
+  cases ty <;> simp_all <;> scalar_tac
+
+@[simp]
+theorem UScalar.pos_add_toNat (h : ¬ ty.isSigned) (x : Scalar ty) (n : Int) (h' : 0 ≤ n) :
+  (n + x.val).toNat = n.toNat + x.val.toNat := by
+  cases ty <;> simp_all <;> scalar_tac
+
+set_option maxHeartbeats 5000000
+
+-- TODO: use simp with discharger to simplify array expressions
+-- TODO: introduce gindex (for ghost index)
+@[pspec]
+theorem add_no_overflow_loop_spec
+  (x : alloc.vec.Vec U32) (y : alloc.vec.Vec U32) (i : Usize)
+  (hLength : x.length = y.length)
+  -- No overflow occurs when we add the individual thunks
+  (hNoOverflow : ∀ (j : Int), i.val ≤ j → j < x.length → (x.val.index j).val + (y.val.index j).val ≤ U32.max)
+  (hi : i.val ≤ x.length) :
+  ∃ x', add_no_overflow_loop x y i = ok x' ∧
+  x'.length = x.length ∧
+  toInt x' = toInt x + 2 ^ (32 * i.toNat) * toInt_aux (y.val.idrop i.val) := by
+  rw [add_no_overflow_loop]
+  simp
+  split
+  . progress as ⟨ yv ⟩
+    progress as ⟨ xv ⟩
+    progress as ⟨ sum ⟩
+    . have := hNoOverflow i.val (by scalar_tac) (by scalar_tac)
+      scalar_tac
+    . progress as ⟨ i' ⟩
+      progress as ⟨ x1 ⟩
+      progress as ⟨ x2 ⟩
+      . -- TODO: this should have been proven by scalar_tac
+        simp_all
+      . intro j h0 h1
+        -- TODO: this is annoying
+        -- TODO: aesop?
+        have : i.val < j := by scalar_tac
+        simp_all
+        apply hNoOverflow j (by scalar_tac) (by scalar_tac)
+      . -- TODO: this should have been proven by scalar_tac
+        simp_all
+        scalar_tac
+      . -- Postcondition
+        have : 0 ≤ i.val := by scalar_tac -- TODO: annoying
+        simp_all [toInt]
+        ring_nf
+  . simp_all
+termination_by (x.length - i.val).toNat
+decreasing_by scalar_decr_tac
+
+/- [tutorial::add_no_overflow]:
+   Source: 'src/lib.rs', lines 18:0-18:50 -/
+def add_no_overflow
+  (x : alloc.vec.Vec U32) (y : alloc.vec.Vec U32) :
+  Result (alloc.vec.Vec U32)
+  :=
+  add_no_overflow_loop x y 0#usize
+
+theorem add_no_overflow_spec (x : alloc.vec.Vec U32) (y : alloc.vec.Vec U32)
+  (hLength : x.length = y.length)
+  (hNoOverflow : ∀ (j : Int), 0 ≤ j → j < x.length → (x.val.index j).val + (y.val.index j).val ≤ U32.max) :
+  ∃ x', add_no_overflow x y = ok x' ∧
+  x'.length = y.length ∧
+  toInt x' = toInt x + toInt y := by
+  rw [add_no_overflow]
+  progress as ⟨ x' ⟩
+  simp_all [toInt]
+
+/- [tutorial::add_with_carry]: loop 0:
+   Source: 'src/lib.rs', lines 39:4-50:1 -/
+divergent def add_with_carry_loop
+  (x : alloc.vec.Vec U32) (y : alloc.vec.Vec U32) (c0 : U8) (i : Usize) :
+  Result (U8 × (alloc.vec.Vec U32))
+  :=
+  let i1 := alloc.vec.Vec.len U32 x
+  if i < i1
+  then
+    do
+    let i2 ←
+      alloc.vec.Vec.index U32 Usize (core.slice.index.SliceIndexUsizeSliceTInst
+        U32) x i
+    let i3 ← Scalar.cast .U32 c0
+    let p ← core.num.U32.overflowing_add i2 i3
+    let (sum, c1) := p
+    let i4 ←
+      alloc.vec.Vec.index U32 Usize (core.slice.index.SliceIndexUsizeSliceTInst
+        U32) y i
+    let p1 ← core.num.U32.overflowing_add sum i4
+    let (sum1, c2) := p1
+    let i5 ← Scalar.cast_bool .U8 c1
+    let i6 ← Scalar.cast_bool .U8 c2
+    let c01 ← i5 + i6
+    let (_, index_mut_back) ←
+      alloc.vec.Vec.index_mut U32 Usize
+        (core.slice.index.SliceIndexUsizeSliceTInst U32) x i
+    let i7 ← i + 1#usize
+    let x1 ← index_mut_back sum1
+    add_with_carry_loop x1 y c01 i7
+  else Result.ok (c0, x)
+
+-- TODO:
+@[pspec]
+theorem Scalar.cast_bool_spec ty (b : Bool) :
+  ∃ s, Scalar.cast_bool ty b = ok s ∧ s.val = if b then 1 else 0 := by
+  simp [Scalar.cast_bool]
+  sorry
+
+-- TODO:
+@[pspec]
+theorem core.num.U32.overflowing_add_spec' (x y : U32) :
+  ∃ z b, core.num.U32.overflowing_add x y = ok (z, b) ∧
+  if x.val + y.val > U32.max then (z.val = x.val + y.val - U32.max - 1 ∧ b = true)
+  else (z.val = x.val + y.val ∧ b = false)
+  := by
+  sorry
+
+@[pspec]
+theorem add_with_carry_loop_spec
+  (x : alloc.vec.Vec U32) (y : alloc.vec.Vec U32) (c0 : U8) (i : Usize)
+  (hLength : x.length = y.length)
+  (hi : i.val ≤ x.length)
+  (hCarryLe : c0.val ≤ 1) :
+  ∃ x' c1, add_with_carry_loop x y c0 i = ok (c1, x') ∧
+  x'.length = x.length ∧
+  c1.val ≤ 1 ∧
+  toInt x' + c1.val * 2 ^ (32 * x'.length) =
+    toInt x + 2 ^ (32 * i.toNat) * toInt_aux (y.val.idrop i.val) + c0.val * 2 ^ (32 * i.toNat) := by
+  rw [add_with_carry_loop]
+  simp
+  split
+  . progress as ⟨ xi ⟩
+    progress as ⟨ c0u ⟩
+    . -- TODO: automation with scalar tac, and more precise lemmas
+      simp
+      scalar_tac
+    . progress as ⟨ s1, c1, hConv1 ⟩
+      progress as ⟨ yi ⟩
+      progress as ⟨ s2, c2, hConv2 ⟩
+      progress as ⟨ c1u ⟩
+      progress as ⟨ c2u ⟩
+      progress as ⟨ c3 ⟩
+      . -- TODO: scalar_tac should have succeeded
+        simp [U8.max]
+        omega
+      . progress as ⟨ _ ⟩
+        progress as ⟨ i1 ⟩
+        progress as ⟨ x1 ⟩
+        progress as ⟨ c4, x2 ⟩
+        . -- TODO: this should have been proven by scalar_tac
+          simp_all
+        . -- TODO: this should have been proven by scalar_tac
+          simp_all
+          scalar_tac
+        . -- TODO: scalar_tac should do all this on its own
+          split at hConv1 <;>
+          split at hConv2 <;>
+          simp_all
+          scalar_tac
+        . simp_all [toInt]
+          have hxUpdate := toInt_aux_update x.val i.val s2 (by scalar_tac) (by scalar_tac)
+          simp [hxUpdate]; clear hxUpdate
+          have hyDrop := toInt_aux_idrop y.val i.val (by scalar_tac) (by scalar_tac)
+          simp [hyDrop]; clear hyDrop
+          ring_nf
+          split at hConv1 <;>
+          split at hConv2 <;>
+          simp_all <;>
+          ring_nf <;> simp [U32.max] <;> ring_nf
+  . simp_all
+    scalar_tac
+termination_by (x.length - i.val).toNat
+decreasing_by scalar_decr_tac
+
+-- TODO: boost ring_nf
+
+/-
+Use scalar_tac here:
+
+x y : alloc.vec.Vec U32
+c0 : U8
+i : Usize
+xi c0u s1 : U32
+c1 : Bool
+yi s2 : U32
+c2 : Bool
+c1u c2u c3 : U8
+x✝ : U32
+i1 : Usize
+x1 : alloc.vec.Vec U32
+hLength : (↑x).length = (↑y).length
+hi : ↑i ≤ ↑(↑y).length
+hCarryLe : ↑c0 ≤ 1
+h✝² : ↑i < ↑(↑y).length
+_✝⁸ : xi = (↑x).index ↑i
+_✝⁷ : ↑c0u = ↑c0
+_✝⁶ : yi = (↑y).index ↑i
+_✝⁵ : ↑c1u = 1
+_✝⁴ : ↑c2u = 1
+_✝³ : ↑c3 = 2
+_✝² : x✝ = (↑x).index ↑i
+_✝¹ : ↑i1 = ↑i + 1
+_✝ : ↑x1 = (↑x).update (↑i) s2
+h✝¹ : U32.max < ↑((↑x).index ↑i) + ↑c0
+hConv1 : ↑s1 = ↑((↑x).index ↑i) + ↑c0 - U32.max - 1 ∧ c1 = true
+h✝ : U32.max < ↑((↑x).index ↑i) + ↑c0 - U32.max - 1 + ↑((↑y).index ↑i)
+hConv2 : ↑s2 = ↑((↑x).index ↑i) + ↑c0 - U32.max - 1 + ↑((↑y).index ↑i) - U32.max - 1 ∧ c2 = true
+-/
+
+-- TODO: improve scalar_tac to do the splits properly
+example (b : Bool) (x y : Int) (h : if b then P ∧ x + y < 3 else x + y < 4) : x + y < 5 := by
+  repeat (split at *) <;>
+  omega
+
+/- [tutorial::add_with_carry]:
+   Source: 'src/lib.rs', lines 37:0-37:55 -/
+def add_with_carry
+  (x : alloc.vec.Vec U32) (y : alloc.vec.Vec U32) :
+  Result (U8 × (alloc.vec.Vec U32))
+  :=
+  add_with_carry_loop x y 0#u8 0#usize
+
+@[pspec]
+theorem add_with_carry_spec
+  (x : alloc.vec.Vec U32) (y : alloc.vec.Vec U32)
+  (hLength : x.length = y.length) :
+  ∃ x' c, add_with_carry x y = ok (c, x') ∧
+  x'.length = x.length ∧
+  c.val ≤ 1 ∧
+  toInt x' + c.val * 2 ^ (32 * x'.length) = toInt x + toInt y := by
+  rw [add_with_carry]
+  progress as ⟨ c, x' ⟩
+  simp_all
+
+/- [tutorial::max]:
+   Source: 'src/lib.rs', lines 26:0-26:37 -/
+def max (x : Usize) (y : Usize) : Result Usize :=
+  if x > y
+  then Result.ok x
+  else Result.ok y
+
+/- [tutorial::get_or_zero]:
+   Source: 'src/lib.rs', lines 30:0-30:45 -/
+def get_or_zero (y : alloc.vec.Vec U32) (i : Usize) : Result U32 :=
+  let i1 := alloc.vec.Vec.len U32 y
+  if i < i1
+  then
+    alloc.vec.Vec.index U32 Usize (core.slice.index.SliceIndexUsizeSliceTInst
+      U32) y i
+  else Result.ok 0#u32
+
+/- [tutorial::add]: loop 0:
+   Source: 'src/lib.rs', lines 60:4-76:1 -/
+divergent def add_loop
+  (x : alloc.vec.Vec U32) (y : alloc.vec.Vec U32) (max1 : Usize) (c0 : U8)
+  (i : Usize) :
+  Result (alloc.vec.Vec U32)
+  :=
+  if i < max1
+  then
+    do
+    let yi ← get_or_zero y i
+    let i1 ←
+      alloc.vec.Vec.index U32 Usize (core.slice.index.SliceIndexUsizeSliceTInst
+        U32) x i
+    let i2 ← Scalar.cast .U32 c0
+    let p ← core.num.U32.overflowing_add i1 i2
+    let (sum, c1) := p
+    let p1 ← core.num.U32.overflowing_add sum yi
+    let (sum1, c2) := p1
+    let i3 ← Scalar.cast_bool .U8 c1
+    let i4 ← Scalar.cast_bool .U8 c2
+    let c01 ← i3 + i4
+    let (_, index_mut_back) ←
+      alloc.vec.Vec.index_mut U32 Usize
+        (core.slice.index.SliceIndexUsizeSliceTInst U32) x i
+    let i5 ← i + 1#usize
+    let x1 ← index_mut_back sum1
+    add_loop x1 y max1 c01 i5
+  else
+    if c0 != 0#u8
+    then do
+         let i1 ← Scalar.cast .U32 c0
+         alloc.vec.Vec.push U32 x i1
+    else Result.ok x
+
+/- [tutorial::add]:
+   Source: 'src/lib.rs', lines 55:0-55:38 -/
+def add
+  (x : alloc.vec.Vec U32) (y : alloc.vec.Vec U32) :
+  Result (alloc.vec.Vec U32)
+  :=
+  do
+  let i := alloc.vec.Vec.len U32 x
+  let i1 := alloc.vec.Vec.len U32 y
+  let max1 ← max i i1
+  let x1 ← alloc.vec.Vec.resize U32 core.clone.CloneU32 x max1 0#u32
+  add_loop x1 y max1 0#u8 0#usize
+
 end Tutorial
